.

src/program_proof/session/gossip.v
@@ -1,29 +1,216 @@
 From Perennial.program_proof.session Require Export session_prelude coq_session.
-From Perennial.program_proof.session Require Export versionVector sort.
+From Perennial.program_proof.session Require Export versionVector sort processClientRequest.
 
 Section heap.
 
+  Definition coq_receiveGossip (s: Server.t) (r: Message.t) : Server.t :=
+    if length (r.(Message.S2S_Gossip_Operations)) =? 0 then
+      s
+    else
+      let focus := (coq_mergeOperations s.(Server.PendingOperations) r.(Message.S2S_Gossip_Operations)) in
+      let loop_init : nat * Server.t :=
+        (0%nat, Server.mk s.(Server.Id) s.(Server.NumberOfServers) s.(Server.UnsatisfiedRequests) s.(Server.VectorClock) s.(Server.OperationsPerformed) s.(Server.MyOperations) focus s.(Server.GossipAcknowledgements))
+      in
+      let loop_step acc e : nat * Server.t :=
+        let '(i, s) := acc in
+        if coq_oneOffVersionVector s.(Server.VectorClock) e.(Operation.VersionVector) then
+          let OperationsPerformed := coq_mergeOperations s.(Server.OperationsPerformed) [e] in
+          let VectorClock := coq_maxTS s.(Server.VectorClock) e.(Operation.VersionVector) in
+          let PendingOperations := coq_deleteAtIndexOperation s.(Server.PendingOperations) i in
+          (i, Server.mk s.(Server.Id) s.(Server.NumberOfServers) s.(Server.UnsatisfiedRequests) s.(Server.VectorClock) OperationsPerformed s.(Server.MyOperations) PendingOperations s.(Server.GossipAcknowledgements))
+        else ((i + 1)%nat, s)
+      in
+      snd (fold_left loop_step focus loop_init).
+
   Context `{hG: !heapGS Σ}.
-  
-  (* Lemma wp_getGossipOperations (sv: u64*u64*Slice.t*Slice.t*Slice.t*Slice.t*Slice.t*Slice.t) (s: Server.t)
-    (serverId: w64) (n: nat) :
+
+  Lemma wp_receiveGossip (sv:tuple_of[u64,u64,Slice.t,Slice.t,Slice.t,Slice.t,Slice.t,Slice.t]) (s: Server.t)
+    (msgv:tuple_of[u64,u64,u64,u64,u64,Slice.t,u64,u64,Slice.t,u64,u64,u64,u64,u64,u64,Slice.t,u64,u64]) (msg: Message.t)
+    (n: nat) c2s s2c len_mo len_ga :
     {{{
-        is_server sv s n 
+        is_server sv s n n n len_mo n len_ga ∗ 
+        is_message msgv msg n c2s s2c ∗
+        ⌜is_sorted s .(Server.PendingOperations)⌝
+    }}}
+      receiveGossip (server_val sv) (message_val msgv)
+    {{{
+        r, RET r;
+        is_server sv (coq_receiveGossip s msg) n n n len_mo n len_ga ∗
+        is_message msgv msg n c2s s2c
+    }}}.
+  Proof.
+    rewrite redefine_server_val redefine_message_val. TypeVector.des sv. TypeVector.des msgv.
+    iIntros "%Φ (H_server & H_message & %H_sorted) HΦ". rewrite /acknowledgeGossip.
+    iDestruct "H_server" as "(%H1 & %H2 & H3 & H4 & %H5 & H6 & H7 & H8 & H9 & %H10)".
+    iDestruct "H_message" as "(%H11 & %H12 & %H13 & %H14 & %H15 & H16 & %H17 & %H18 & %H19 & H20 & %H21 & %H22 & %H23 & %H24 & %H25 & %H26 & H27 & %H28 & %H29 & %H30)".
+    simplNotation. subst. rewrite /receiveGossip.
+    wp_pures. wp_apply wp_slice_len. wp_if_destruct.
+    - iModIntro. iApply "HΦ". simpl. unfold coq_receiveGossip.
+      destruct (length msg .(Message.S2S_Gossip_Operations) =? 0) as [ | ] eqn: H_OBS.
+      + rewrite Z.eqb_eq in H_OBS. iFrame. simpl. iPureIntro. done.
+      + rewrite Z.eqb_neq in H_OBS. iDestruct "H20" as "(%ops & H1_20 & H2_20)".
+        iPoseProof (own_slice_sz with "[$H1_20]") as "%YES1".
+        iPoseProof (big_sepL2_length with "[$H2_20]") as "%YES2".
+        word.
+    - replace ((#s .(Server.Id), (#s .(Server.NumberOfServers), (t4, (t3, (t2, (t1, (t0, (t, #())))))))))%V with (@SessionPrelude.value_of (tuple_of[u64,u64,Slice.t,Slice.t,Slice.t,Slice.t,Slice.t,Slice.t]) _ (s .(Server.Id), s .(Server.NumberOfServers), t4, t3, t2, t1, t0, t)) by reflexivity. rewrite <- redefine_server_val. simplNotation.
+      wp_apply wp_ref_to. { repeat econstructor; eauto. } rewrite redefine_server_val. simplNotation. iIntros "%server H_server".
+      wp_pures. wp_load. wp_apply (wp_mergeOperations with "[$H8 $H20]"); auto. iIntros "%ns (%nxs & H31 & -> & H8 & H20 & %H2_sorted)".
+      wp_apply (wp_storeField_struct with "[H_server]"). { repeat constructor; auto. } { iExact "H_server". }
+      simpl. iIntros "H_server". wp_pures. wp_apply wp_ref_to; auto. iIntros "%i H_i". wp_pures.
+      rename t4 into UnsatisfiedRequests, t3 into VectorClock, t2 into OperationsPerformed, t1 into MyOperations, t0 into PendingOperations, t into GossipAcknowledgements.
+      set (focus := coq_mergeOperations s .(Server.PendingOperations) msg .(Message.S2S_Gossip_Operations)) in H2_sorted |- *.
+      set (loop_init := (0%nat, Server.mk s.(Server.Id) s.(Server.NumberOfServers) s.(Server.UnsatisfiedRequests) s.(Server.VectorClock) s.(Server.OperationsPerformed) s.(Server.MyOperations) focus s.(Server.GossipAcknowledgements))).
+      set (loop_step := λ (acc : nat * Server.t) (e : Operation.t),
+        let '(i, s) := acc in
+        if coq_oneOffVersionVector s.(Server.VectorClock) e.(Operation.VersionVector) then
+          let OperationsPerformed := coq_mergeOperations s.(Server.OperationsPerformed) [e] in
+          let VectorClock := coq_maxTS s.(Server.VectorClock) e.(Operation.VersionVector) in
+          let PendingOperations := coq_deleteAtIndexOperation s.(Server.PendingOperations) i in
+          (i, Server.mk s.(Server.Id) s.(Server.NumberOfServers) s.(Server.UnsatisfiedRequests) s.(Server.VectorClock) OperationsPerformed s.(Server.MyOperations) PendingOperations s.(Server.GossipAcknowledgements))
+        else ((i + 1)%nat, s)
+      ).
+      set (n := length s .(Server.VectorClock)). rename s into s0.
+      wp_apply (wp_forBreak_cond
+        ( λ continue, ∃ prevs : list Operation.t, ∃ nexts : list Operation.t, ∃ index : nat, ∃ s : Server.t,
+          ⌜focus = prevs ++ nexts⌝ ∗
+          ⌜(index, s) = fold_left loop_step prevs loop_init⌝ ∗
+          i ↦[uint64T] #index ∗
+          server ↦[struct.t Server] (#s .(Server.Id), (#s .(Server.NumberOfServers), (UnsatisfiedRequests, (VectorClock, (OperationsPerformed, (MyOperations, (PendingOperations, (GossipAcknowledgements, #())))))))) ∗
+          message_slice UnsatisfiedRequests s .(Server.UnsatisfiedRequests) n ∗
+          own_slice_small VectorClock uint64T (DfracOwn 1) s .(Server.VectorClock) ∗
+          operation_slice OperationsPerformed s .(Server.OperationsPerformed) n ∗
+          operation_slice MyOperations s .(Server.MyOperations) len_mo ∗
+          operation_slice PendingOperations s .(Server.PendingOperations) n ∗
+          own_slice_small GossipAcknowledgements uint64T (DfracOwn 1) s .(Server.GossipAcknowledgements) ∗
+          own_slice_small t7 uint64T (DfracOwn 1) msg .(Message.C2S_Client_VersionVector) ∗
+          operation_slice t6 msg .(Message.S2S_Gossip_Operations) n ∗
+          own_slice_small t5 uint64T (DfracOwn 1) msg .(Message.S2C_Client_VersionVector) ∗
+          operation_slice ns focus n ∗
+          ⌜length s .(Server.PendingOperations) = (index + length nexts)%nat⌝ ∗
+          ⌜drop index s .(Server.PendingOperations) = nexts⌝ ∗
+          ⌜length s .(Server.VectorClock) = length s0 .(Server.VectorClock)⌝ ∗
+          ⌜is_sorted s .(Server.OperationsPerformed)⌝ ∗
+          ⌜continue = false -> nexts = []⌝
+        )%I
+      with "[] [H_i H_server H3 H4 H6 H7 H8 H9 H16 H20 H27 H31]").
+      { clear Φ. iIntros "%Φ". iModIntro. iIntros "(%prev & %nexts & %index & %s & %H_split_focus & %H_loop & H_i & H_server & H3 & H4 & H6 & H7 & H8 & H20 & H9 & H16 & H27 & H31 & %H_length & %H_nexts & %H1_invariant & %H2_invariant & %H_continue) HΦ".
+        wp_pures. wp_load. wp_load. wp_pures. wp_apply wp_slice_len. wp_if_destruct.
+        - wp_pures. wp_load. wp_pures. wp_load. wp_pures. iDestruct "H8" as "(%ops1 & [H1_8 H2_8] & H3_8)".
+          iPoseProof (big_sepL2_length with "[$H3_8]") as "%YES1".
+          iPoseProof (own_slice_small_sz with "[$H1_8]") as "%YES2".
+          assert (is_Some (ops1 !! uint.nat (W64 index))) as [e H_e].
+          { eapply lookup_lt_is_Some_2. word. }
+          assert (length nexts > 0)%nat as NE_NIL by word.
+          destruct nexts as [ | cur nexts].
+          { simpl in NE_NIL. word. }
+          clear NE_NIL H_continue.
+          assert (s .(Server.PendingOperations) !! index = Some cur) as H_cur.
+          { rewrite <- take_drop with (l := s .(Server.PendingOperations)) (i := index). rewrite lookup_app_r.
+            - rewrite H_nexts. replace (index - length (take index s .(Server.PendingOperations)))%nat with 0%nat.
+              + reflexivity.
+              + symmetry. rewrite length_take. word.
+            - rewrite length_take. word.
+          }
+          wp_apply (wp_SliceGet with "[$H1_8]"); auto. iIntros "H1_8". wp_pures. wp_load. wp_pures.
+          iPoseProof (pers_big_sepL2_is_operation with "[$H3_8]") as "#H3_8_pers".
+          replace (uint.nat (W64 index)) with index in H_e by word.
+          iPoseProof (big_sepL2_is_operation_elim with "[$H3_8_pers]") as "(%op2 & %H1_op2 & H2_op2)"; eauto.
+          iPoseProof (own_slice_small_sz with "[$H4]") as "%YES3".
+          wp_apply (wp_oneOffVersionVector with "[$H4 $H2_op2]"). { iPureIntro. rewrite <- H1_op2. exact H1_invariant. }
+          iIntros "%b (-> & H4 & H2_op2' & %H_length')". wp_if_destruct.
+          + wp_pures. wp_load. wp_pures. wp_load. wp_pures. wp_apply (wp_SliceGet with "[$H1_8]"). { replace (uint.nat (W64 index)) with index by word. iPureIntro. exact H_e. }
+            iIntros "H1_8". wp_apply (wp_SliceSingleton). iIntros "%s1 H_s1". wp_pures. wp_load. wp_pures.
+            wp_apply (wp_mergeOperations with "[$H6 $H_s1]").
+            { instantiate (1 := [cur]). iSplit.
+              - simpl. iSplit; trivial. iApply (big_sepL2_is_operation_elim with "[$H3_8_pers]"); eauto.
+              - iPureIntro. done.
+            }
+            iIntros "%ns' (%nxs & H_ns' & -> & H6 & H_s1 & H3_sorted)".
+            wp_apply (wp_storeField_struct with "[$H_server]"). { repeat econstructor; eauto. } iIntros "H_server".
+            wp_load. wp_pures. wp_load. wp_apply (wp_SliceGet with "[$H1_8]"). { replace (uint.nat (W64 index)) with index by word. iPureIntro. exact H_e. }
+            iIntros "H1_8". wp_pures. wp_load. wp_pures. admit.
+          + admit.
+        - admit.
+      }
+      { admit.
+      }
+      { admit.
+      }
+  Admitted.
+
+  Lemma wp_acknowledgeGossip (sv:tuple_of[u64,u64,Slice.t,Slice.t,Slice.t,Slice.t,Slice.t,Slice.t]) (s: Server.t)
+    (msgv:tuple_of[u64,u64,u64,u64,u64,Slice.t,u64,u64,Slice.t,u64,u64,u64,u64,u64,u64,Slice.t,u64,u64]) (msg: Message.t)
+    (n: nat) c2s s2c len_vc len_op len_mo len_po len_ga :
+    {{{
+        is_server sv s n len_vc len_op len_mo len_po len_ga ∗ 
+        is_message msgv msg n c2s s2c
+    }}}
+      acknowledgeGossip (server_val sv) (message_val msgv)
+    {{{
+        r, RET r;
+        is_server sv (coq_acknowledgeGossip s msg) n len_vc len_op len_mo len_po len_ga ∗
+        is_message msgv msg n c2s s2c
+    }}}.
+  Proof.
+    TypeVector.des sv. TypeVector.des msgv.
+    iIntros "%Φ (H_server & H_message) HΦ". rewrite /acknowledgeGossip.
+    iDestruct "H_server" as "(%H1 & %H2 & H3 & H4 & %H5 & H6 & H7 & H8 & H9 & %H10)".
+    iDestruct "H_message" as "(%H11 & %H12 & %H13 & %H14 & %H15 & H16 & %H17 & %H18 & %H19 & H20 & %H21 & %H22 & %H23 & %H24 & %H25 & %H26 & H27 & %H28 & %H29 & %H30)".
+    simplNotation. subst. rewrite redefine_message_val redefine_server_val. simpl in *. wp_pures.
+    wp_apply (wp_slice_len). wp_if_destruct.
+    - iModIntro. iApply "HΦ". unfold coq_acknowledgeGossip.
+      destruct (uint.Z msg .(Message.S2S_Acknowledge_Gossip_Sending_ServerId) >=? length s .(Server.GossipAcknowledgements)) as [ | ] eqn: H_OBS; simpl.
+      + iFrame. iPureIntro. done.
+      + rewrite Z.geb_leb in H_OBS. rewrite Z.leb_gt in H_OBS.
+        iPoseProof (own_slice_small_sz with "[$H9]") as "%YES1".
+        word.
+    - iPoseProof (own_slice_small_sz with "[$H9]") as "%YES2".
+      assert (uint.nat msg .(Message.S2S_Acknowledge_Gossip_Sending_ServerId) < length s.(Server.GossipAcknowledgements))%nat as YES1 by word.
+      apply list_lookup_lt in YES1. destruct YES1 as [x H_x].
+      wp_apply (wp_SliceGet with "[$H9]"); auto. iIntros "H9". wp_apply (wp_maxTwoInts with "[]"); auto.
+      iIntros "%r ->". wp_apply (slice.wp_SliceSet with "[H9]").
+      { iSplitL "H9".
+        - iExact "H9".
+        - iPureIntro. split; auto.
+          exists (u64_IntoVal.(to_val) x). cbn.
+          rewrite list_lookup_fmap. rewrite H_x. done.
+      }
+      iIntros "H9". wp_pures. iModIntro. iApply "HΦ". iFrame. iSplitR "".
+      + unfold is_server. simplNotation. unfold coq_acknowledgeGossip.
+        destruct (uint.Z msg .(Message.S2S_Acknowledge_Gossip_Sending_ServerId) >=? length s .(Server.GossipAcknowledgements)) as [ | ] eqn: H_OBS.
+        * rewrite Z.geb_ge in H_OBS. word.
+        * rewrite H_x. simpl. iFrame.
+          iSplitL "". { done. }
+          iSplitL "". { done. }
+          iSplitL "". { done. }
+          iSplitL "H9".
+          { unfold own_slice_small. unfold list.untype. cbn. rewrite list_fmap_insert. done. }
+          { rewrite length_insert. done. }
+      + iPureIntro. done.
+  Qed.
+
+  Lemma wp_getGossipOperations (sv:tuple_of[u64,u64,Slice.t,Slice.t,Slice.t,Slice.t,Slice.t,Slice.t]) (s: Server.t)
+    (serverId: w64) (n: nat) len_vc len_op len_mo len_po len_ga :
+    {{{
+        is_server sv s n len_vc len_op len_mo len_po len_ga
     }}}
       getGossipOperations (server_val sv) #serverId
     {{{
         ns , RET slice_val (ns);
-        operation_slice ns (coq_getGossipOperations s serverId) n ∗
-        is_server sv s n 
+        operation_slice ns (coq_getGossipOperations s serverId) len_mo ∗
+        is_server sv s n len_vc len_op len_mo len_po len_ga
     }}}.
   Proof.
-    iIntros "%Φ (%H1 & %H2 & H3 & %H4 & H5 & H6 & H7 & H8 & %H9 & H10) HΦ". rewrite /getGossipOperations. wp_pures.
+    TypeVector.des sv.
+    iIntros "%Φ (%H1 & %H2 & H3 & H4 & %H5 & H6 & H7 & H8 & H9 & %H10) HΦ".
+    simplNotation. subst.
+    rewrite /getGossipOperations. wp_pures.
     wp_apply wp_NewSlice; auto. iIntros "%s1 [H1_s1 H2_s1]".
     iPoseProof (own_slice_small_sz with "[$H1_s1]") as "%H_s1_len".
-    iPoseProof (own_slice_small_sz with "[$H10]") as "%YES1".
-    iPoseProof (own_slice_small_sz with "[$H5]") as "%YES2".
+    iPoseProof (own_slice_small_sz with "[$H9]") as "%YES1".
+    iPoseProof (own_slice_small_sz with "[$H4]") as "%YES2".
     wp_apply wp_ref_to; auto. iIntros "%ret H_ret".
-    wp_pures. wp_bind (if: #serverId ≥ slice.len sv.2 then #true else _)%E.
+    wp_pures. wp_bind (if: #serverId ≥ slice.len t then #true else _)%E.
     wp_apply wp_slice_len; auto. wp_if_destruct.
     - wp_pures. wp_load. iModIntro. iApply "HΦ". iFrame.
       replace (replicate (uint.nat (W64 0)) operation_into_val .(IntoVal_def (Slice.t * w64))) with (@nil (Slice.t * w64)) in *; simpl in *; trivial. iSplitL "".
@@ -34,25 +221,26 @@ Section heap.
     - wp_pures. wp_apply wp_slice_len; auto.
       assert (is_Some (s .(Server.GossipAcknowledgements) !! uint.nat serverId)) as [v H_v].
       { eapply lookup_lt_is_Some_2. word. }
-      wp_apply (wp_SliceGet with "[$H10]"); auto.
+      wp_apply (wp_SliceGet with "[$H9]"); auto.
       iIntros "H1". simpl. wp_pures. wp_if_destruct.
-      + wp_load. iModIntro. iApply "HΦ". iDestruct "H7" as "[%ops [H7 H4]]".
+      + wp_load. iModIntro. iApply "HΦ". iDestruct "H7" as "[%ops [H7 H9]]". unfold tuple_of in *. simpl in *.
         iPoseProof (own_slice_sz with "[$H7]") as "%YES3".
-        iPoseProof (big_sepL2_length with "[$H4]") as "%YES4".
+        iPoseProof (big_sepL2_length with "[$H9]") as "%YES4".
         iFrame. simpl in *. replace (replicate (uint.nat (W64 0)) (Slice.nil, W64 0)) with (@nil (Slice.t * w64)) in *; simpl in *; trivial. iSplitL "".
         * unfold coq_getGossipOperations. rewrite H_v. rewrite skipn_all2.
           { simpl. done. }
           { word. }
         * iPureIntro. tauto.
-      + wp_pures. wp_apply (wp_SliceGet with "[$H1]"); auto. iIntros "H9". simpl in *.
-        wp_pures. wp_apply wp_SliceSkip; auto. { word. } wp_load. iDestruct "H7" as "(%ops & [H7 H10] & H4)".
+      + rewrite redefine_server_val. simpl. wp_pures.
+        wp_apply (wp_SliceGet with "[$H1]"); auto. iIntros "H9". simpl in *.
+        wp_pures. wp_apply wp_SliceSkip; auto. { word. } wp_load. iDestruct "H7" as "(%ops & [H7 H10] & H11)".
         iPoseProof (own_slice_small_sz with "[$H7]") as "%YES3".
-        iPoseProof (big_sepL2_length with "[$H4]") as "%YES4".
+        iPoseProof (big_sepL2_length with "[$H11]") as "%YES4".
         iPoseProof (slice_small_split with "[$H7]") as "[H7 H7']".
         { instantiate (1 := v). word. }
         wp_apply (wp_SliceAppendSlice with "[$H1_s1 $H2_s1 H7']"); auto.
         iIntros "%s2 [H1_s2 H2_s2]". replace (replicate (uint.nat (W64 0)) (Slice.nil, W64 0)) with (@nil (Slice.t * w64)) in * by reflexivity. simpl in *.
-        iApply "HΦ". iPoseProof (pers_big_sepL2_is_operation with "[$H4]") as "#H10_pers". iFrame.
+        iApply "HΦ". iPoseProof (pers_big_sepL2_is_operation with "[$H11]") as "#H10_pers". iFrame.
         iSplitL "".
         { unfold coq_getGossipOperations. rewrite H_v. rewrite <- take_drop with (l := ops) (i := uint.nat v) at 1. rewrite <- take_drop with (l := s.(Server.MyOperations)) (i := uint.nat v) at 1.
           iPoseProof (big_sepL2_app_equiv with "[$H10_pers]") as "[YES1 YES2]".
@@ -64,90 +252,10 @@ Section heap.
         iSplitL "". { iPureIntro. tauto. }
         iSplitR "".
         { iApply own_slice_small_take_drop.
-          - instantiate (1 := v). word.
+          - instantiate (1 := v). simplNotation. word.
           - iFrame.
         }
         iPureIntro. tauto.
   Qed.
-
-  Lemma wp_acknowledgeGossip (sv: u64*u64*Slice.t*Slice.t*Slice.t*Slice.t*Slice.t*Slice.t) (s: Server.t)
-    (msgv: u64*u64*u64*u64*u64*Slice.t*u64*u64*Slice.t*u64*u64*u64*u64*u64*u64*Slice.t*u64*u64)
-    (msg: Message.t) (n: nat) c2s s2c :
-    {{{
-          is_server sv s n ∗ 
-          is_message' msgv msg n c2s s2c
-    }}}
-      acknowledgeGossip (server_val sv) (message_val msgv)
-      {{{
-            r , RET r;
-            is_server sv (coq_acknowledgeGossip s msg) n ∗
-            ∃ a, ∃ b, is_message' msgv msg n a b
-      }}}.
-  Proof.
-    iIntros "%Φ (H1 & H2) H_ret".
-    rewrite /acknowledgeGossip.
-    iDestruct "H1" as "(%H1 & %H2 & H1 & %H3 & H4 & H5 & H6 & H7 & %H4 & H8)".
-    iDestruct "H2" as "(%H5 & %H6 & %H7 & %H8 & %H9 & %H10 & H9 & %H11 & %H12 & H10 & %H13 & %H14 & %H15 & %H16 & %H17 & %H18 & %H19 & H11 & %H20 & %H21)".
-    wp_pures.
-    wp_apply (wp_slice_len).
-    iDestruct (own_slice_small_sz with "H8") as "%H22". 
-    wp_if_destruct.
-    { iModIntro. iApply "H_ret". iFrame.
-    assert (uint.Z msg.(Message.S2S_Acknowledge_Gossip_Sending_ServerId) >=? length s.(Server.GossipAcknowledgements) = true) by word.
-      iSplitL.
-      - unfold coq_acknowledgeGossip.
-        rewrite H. iFrame. iPureIntro.
-        repeat split; auto.
-      - iPureIntro. repeat split; auto.
-    } 
-    assert (uint.nat msgv.1.1.1.1.1.1.1.2 < length s.(Server.GossipAcknowledgements))%nat
-      by word.
-    apply list_lookup_lt in H as [x H].
-    wp_apply (wp_SliceGet with "[H8]"). { iFrame. auto. }
-    iIntros "H8".
-    wp_apply (wp_maxTwoInts with "[]"). { auto. }
-    iIntros (r) "%H23".
-    wp_pures.
-    rewrite H23.
-    wp_apply (slice.wp_SliceSet with "[H8]"). { iSplitL "H8".
-                                                - iApply "H8".
-                                                - iPureIntro. split; auto.
-                                                  unfold is_Some.
-                                                  exists (u64_IntoVal.(to_val) x).
-                                                  simpl. unfold list.untype.
-                                                  simpl. rewrite list_lookup_fmap.
-                                                  rewrite H. auto. }
-    iIntros "H". wp_pures. iModIntro.
-    iApply "H_ret".
-    iSplitL "H H1 H4 H5 H6 H7".
-    - unfold coq_acknowledgeGossip.
-      assert (uint.Z msg.(Message.S2S_Acknowledge_Gossip_Sending_ServerId) >=?
-                           length s.(Server.GossipAcknowledgements) = false) by word.
-      rewrite H0. 
-      iSplit. { auto. }
-      iSplit. { auto. }
-      iSplitL "H1". { auto. }
-      iSplit. { auto. }
-      iSplitL "H4". { auto. }
-      iSplitL "H5". { auto. }
-      iSplitL "H6". { auto. }
-      iSplitL "H7". { auto. }
-      iSplit. { simpl. iPureIntro.
-                rewrite length_insert. auto. }
-      simpl.
-      rewrite <- H14.
-      rewrite H. 
-      unfold own_slice_small.
-      assert ((<[uint.nat msgv.1.1.1.1.1.1.1.2:=#(coq_maxTwoInts x msgv.1.1.1.1.1.2)]>
-                 (list.untype s.(Server.GossipAcknowledgements))) =
-              (list.untype
-                 (<[uint.nat msgv.1.1.1.1.1.1.1.2:=coq_maxTwoInts x msg.(Message.S2S_Acknowledge_Gossip_Index)]>
-                    s.(Server.GossipAcknowledgements)))).
-      { unfold list.untype. rewrite list_fmap_insert. simpl. rewrite H16. auto. }
-      rewrite H24. iFrame.
-    - unfold is_message. iFrame.
-      iPureIntro.
-      repeat split; auto.
-  Qed. *)
 
 End heap.
